\documentclass{article}
\usepackage[utf8]{inputenc}
\usepackage{circuitikz}
\title{Assignment 6}
\author{mahesh}
\begin{document}
\maketitle

  \section{ question}
    
       The expression $ \sim(p \leftrightarrow q)$   is equivalent to:
       
  \section{answer}
   $ \to  \sim (p\leftrightarrow q) $
   
    $ \to  \sim {(p\longrightarrow q)\bigwedge(q \longrightarrow p)}$ 
    
    $ \to  { \sim(p \longrightarrow q) \bigvee \sim(q\longrightarrow p) }$
    
BY DEMORGAN'S LAW;

   ${(p \bigwedge  \sim q) \bigvee (q \bigwedge \sim p) }$
 
  Hence proved that
 
 $ \sim(p \leftrightarrow q) \equiv    {(p \bigwedge  \sim q) \bigvee (q \bigwedge \sim p) }$
 
 \section{conversion to AND and OR gates} 
  $\to  \sim(p \leftrightarrow q)\equiv    {(p \bigwedge  \sim q) \bigvee (q \bigwedge \sim p) }$
  
 
  $\to  \sim(p \leftrightarrow q)\equiv  p.\overline{q} + q.\overline{p}$
  
  
\begin{figure}[h]
\centering
\begin{circuitikz}
\ctikzset{logic ports origin=center};
 \draw
 (0,0)node[and port](myand1){}
 (0,4)node[and port](myand2){}
 (2,2)node[or port](myor){}

 (myand1.bin 2) node[ocirc, left]{}
 (myand2.bin 1) node[ocirc, left]{}
 

 (myand1.in 1) node[anchor=east] {p}
 (myand1.in 2) node[anchor=east] {q}
 (myand2.in 1) node[anchor=east] {p}
 (myand2.in 2) node[anchor=east] {q}
 (myor.out) node[anchor=west] {Y}
 
 (myand1.out)--(myor.in 1){}
 (myand2.out)--(myor.in 2){};
 
\end{circuitikz}
\caption{Logic Gate }
\label{fig:my_label}
\end{figure}
 
\begin{equation} 
Y=p.\overline{q} + q.\overline{p}
\end{equation}

\end{document}
